add working implementation

complete-theory/compositionalityScript.sml
@@ -7,15 +7,12 @@ val _ = add_rule
   pp_elements = [TOK "(", TM, TOK ",", TM, TOK ")"], paren_style = OnlyIfNecessary,
   block_style = (AroundEachPhrase, (PP.INCONSISTENT, 2))};
 
-val _ = add_rule
-  {term_name = "Interpretation_S", fixity = Closefix,
-  pp_elements = [TOK "⟨", TM, TOK "⟩MS"], paren_style = OnlyIfNecessary,
-  block_style = (AroundEachPhrase, (PP.INCONSISTENT, 2))};
-
+(*
 val _ = add_rule
   {term_name = "Assertional", fixity = Closefix,
   pp_elements = [TOK "Assertional(", TM, TOK ")"], paren_style = OnlyIfNecessary,
   block_style = (AroundEachPhrase, (PP.INCONSISTENT, 2))};
+*)
 
 val _ = add_rule {block_style = (AroundEachPhrase, (PP.INCONSISTENT, 2)),
                   fixity = Infix(NONASSOC, 425),
@@ -48,40 +45,41 @@ val _ = add_rule {block_style = (AroundEachPhrase, (PP.INCONSISTENT, 2)),
                   term_name = "Composition"}
 
 Datatype:
-  C = Q α | Composition C C
-End
-
-Datatype:
-  S = P (α set) | And S S | Contract S S | Parallell S S | Assertional S
+  Term = Impl C S | Assertional S | Refines S S ;
+  C    = Q α | Composition C C ;
+  S    = P (α set) | And S S | Contract S S | Parallell S S
 End
 
 Definition C_M:
-    C_M (Q α) = {α}
+    C_M (Q α)     = {α}
   ∧ C_M (c1 ₓ c2) = (C_M c1) ∩ (C_M c2)
 End
 
-(* TODO Contract, Parallell *)
-Definition Interpretation:
-    (S_M (P α) = {α})
-  ∧ (S_M (And s1 s2) = (S_M s1) ∩ (S_M s2))
-  ∧ (S_M (Contract s1 s2) = {b | ∀b'. b' ∈ S_M s1 ⇒ b' ∩ b ∈ S_M s2})
+Definition S_M:
+    (S_M (P α)             = {α})
+  ∧ (S_M (And s1 s2)       = (S_M s1) ∩ (S_M s2))
+  ∧ (S_M (Contract s1 s2)  = {b | ∀b'. C_M b' ∈ S_M s1 ⇒ C_M b' ∩ b ∈ S_M s2})
   ∧ (S_M (Parallell s1 s2) = {a ∩ b | a ∈ (S_M s1) ∧ b ∈ (S_M s2)})
-  ∧ (S_M (Assertional s) = S_M s)
 End
 
-Definition Impl:
-    (Impl (c:α C) (s:α S) = if C_M c ∈ S_M s then T else F)
-End
-
-Definition Refines:
-  Refines (s1:α S) (s2:α S) = if S_M s1 ⊆ S_M s2 then T else F
+Definition T_M:
+    (T_M (Impl c s)      ⇔ C_M c ∈ S_M s)
+  ∧ (T_M (Refines s1 s2) ⇔ S_M s1 ⊆ S_M s2)
 End
 
 Theorem IMPL_AX_THM:
-  ∀c s. C_M c ∈ S_M s ⇔ Impl c s
+  ∀c s. T_M (Impl c s) ⇔ C_M c ∈ S_M s 
 Proof
   EVAL_TAC >>
   rw[]
+QED
+
+Theorem COMP_ASSOC_THM:
+  ∀c1 c2 c3 s. T_M (Impl (Composition (Composition c1 c2) c3) s) ⇔ T_M (Impl (Composition c1 (Composition c2 c3)) s)
+Proof
+  EVAL_TAC >>
+  rw[] >>
+  metis_tac[pred_setTheory.INTER_ASSOC]
 QED
 
 Theorem ELEM_IN_AND_THM:
@@ -92,71 +90,113 @@ Proof
 QED
 
 Theorem AND_THM:
-  ∀c s1 s2. Impl c s1 ∧ Impl c s2 ⇒ Impl c (And s1 s2)
+  ∀c s1 s2. T_M (Impl c s1) ∧ T_M (Impl c s2) ⇒ T_M (Impl c (And s1 s2))
 Proof
   rw[] >>
   metis_tac[IMPL_AX_THM, ELEM_IN_AND_THM]
 QED
 
 Theorem AND_ELIM_1_THM:
-  ∀c s1 s2. Impl c (And s1 s2) ⇒ Impl c s2
+  ∀c s1 s2. T_M (Impl c (And s1 s2)) ⇒ T_M (Impl c s2)
 Proof
   EVAL_TAC >>
   rw[]
 QED
 
 Theorem AND_ELIM_2_THM:
-  ∀c s1 s2. Impl c (And s1 s2) ⇒ Impl c s1
-Proof
-  EVAL_TAC >>
-  rw[]
-QED
-
-Theorem CONTRACT_ELIM_THM:
-  ∀c1 c2 s1 s2. Impl c1 s1 ∧ Impl c2 (s1, s2) ⇒ Impl (Composition c1 c2) s2
-Proof
-  EVAL_TAC >>
-  rw[]
-QED
-
-Theorem SPEC_CONTRACT_INTRO_THM:
-  ∀c2 s1 s2. (∀q0. q0 ∈ S_M s1 ⇒ (q0 ∩ C_M c2) ∈ S_M s2) ⇒ Impl c2 (s1,s2)
+  ∀c s1 s2. T_M (Impl c (And s1 s2)) ⇒ T_M (Impl c s1)
 Proof
   EVAL_TAC >>
   rw[]
 QED
 
 Theorem REFINEMENT_THM:
-  ∀c s1 s2. Impl c s1 ∧ Refines s1 s2 ⇒ Impl c s2
+  ∀c s1 s2. T_M (Impl c s1) ∧ T_M (Refines s1 s2) ⇒ T_M (Impl c s2)
 Proof
   EVAL_TAC >>
   metis_tac[pred_setTheory.SUBSET_DEF, pred_setTheory.SUBSET_TRANS]
 QED
 
-(*
-Theorem CONTRACT_INTRO_THM:
-  ∀c2 s1 s2. (∀c1. Impl c1 s1 ⇒ Impl (Composition c1 c2) s2) ⇒ Impl c2 (s1,s2)
+Theorem CONTRACT_ELIM_THM:
+  ∀c1 c2 s1 s2. T_M (Impl c1 s1) ∧ T_M(Impl c2 (s1, s2)) ⇒ T_M (Impl (Composition c1 c2) s2)
 Proof
-  EVAL_TAC
+  EVAL_TAC >>
   rw[]
+QED
 
+Theorem SPEC_CONTRACT_INTRO_THM:
+  ∀c2 s1 s2. (∀q0. T_M (Impl q0 s1) ⇒ T_M (Impl (Composition q0 c2) s2)) ⇒ T_M (Impl c2 (s1,s2))
+Proof
+  EVAL_TAC >>
+  rw[]
+QED
+
+(*
+define new and operator as part of term grammar
+*)
+
+Inductive G:
+    (∀(t:α Term) Γ. (t <: Γ) ⇒ G Γ t) (* ax *)
+  ∧ (∀t1 t2 Γ. G Γ t1 ∧ (T_M t1 ⇒ T_M t2) ⇒ G Γ t2) (* lower-level-imp *)
+  ∧ (∀q0 c s1 s2 Γ. G (BAG_INSERT (Impl q0 s1) Γ) (Impl (Composition q0 c) s2) ⇒ G Γ (Impl c (s1, s2))) (* contract *)
+  ∧ (∀c1 c2 s Γ. G Γ (Impl c1 s) ∧ BAG_IN (Assertional s) Γ ⇒ G Γ (Impl (Composition c1 c2) s)) 
+  ∧ (∀t1 t2 Γ . G Γ t1 ⇒ G (BAG_INSERT t2 Γ) t1) (* closure *)
+End
+
+val [G_AX, G_LOWER_IMP, G_CONTRACT_AX, G_ASSERTION, G_CLOSURE] = CONJUNCTS G_rules;
+
+Theorem G_REFINEMENT_THM:
+  ∀c s1 s2 Γ. G Γ ((Impl c s1)) ∧ (BAG_IN (Refines s1 s2) Γ) ⇒ G Γ (Impl c s2)
+Proof
+  rw[] >>
+  ‘G Γ (Refines s1 s2)’ by metis_tac[G_AX] >>
+  ASSUME_TAC REFINEMENT_THM >>
+  metis_tac[G_LOWER_IMP] >>
+  metis_tac[G_AX, REFINEMENT_THM, G_LOWER_IMP]
+QED
+
+(*
+Theorem G_CONTRACT_INTRO_THM:
+  ∀q0 c s1 s2 Γ. G ((Impl q0 s1) INSERT Γ) (Impl (Composition q0 c) s2) ⇒ G Γ (Impl c (s1, s2))
+Proof
+  rw[]
+  ‘G ((Impl q0 s1) INSERT Γ) (Impl q0 s1)’ by metis_tac[G_AX, pred_setTheory.IN_INSERT]
+  ASSUME_TAC SPEC_CONTRACT_INTRO_THM
+  metis_tac[G_LOWER_IMP]
 QED
 *)
+
+val comp_rules = [ELEM_IN_AND_THM,
+                  AND_THM,
+                  AND_ELIM_1_THM,
+                  AND_ELIM_2_THM,
+                  CONTRACT_ELIM_THM,
+                  SPEC_CONTRACT_INTRO_THM,
+                  REFINEMENT_THM,
+                  G_AX,
+                  G_LOWER_IMP,
+                  G_CONTRACT_AX,
+                  G_ASSERTION,
+                  G_REFINEMENT_THM,
+                  G_CLOSURE,
+                  BAG_IN_BAG_INSERT,
+                  COMP_ASSOC_THM];
+
 
 (*
 Context menu
 
 Pallet
-        
-ax
-and-introduction
-and-elimination-1
-and-elimination-2
-contract-introduction
-contract-elimination
-assertional
-refinement
 *)
 
+Theorem TEST:
+  let
+    Γ = {|Assertional a; Refines a a1; Refines (And a g1) a2; Refines g2 g|}
+  in
+    G Γ (Impl c1 (a1, g1)) ∧ G Γ (Impl c2 (a2, g2)) ⇒ G Γ (Impl (Composition c1 c2) (a, g))
+Proof
+  rw[] >>
+  ‘G {|Assertional a; Refines a a1; Refines (And a g1) a2; Refines g2 g|} (Impl (Composition c1 c2) (a, g))’ by metis_tac comp_rules
+QED
 
 val _ = export_theory();
